introduce "set of executable addresses"
Eventually this will allow to describe ifence, but at the moment we just
use too restrictive RiscvProgram instances which fail if a program tries
to fetch an instruction from a previously written address, so by proving
our software correct against this model, we prove that our software will
also run correctly on any processor with instruction caching.

src/Platform/RiscvMachine.v
@@ -17,41 +17,109 @@ Section Machine.
   (* (memory before call, call name, arg values) and (memory after call, return values) *)
   Definition LogItem: Type := (Mem * string * list word) * (Mem * list word).
 
+  (* set of executable addresses. On some processors, this could be the whole address range,
+     while on others, only a specific range. And when an address is written, we might
+     conservatively remove it from that set if we want to prove that our software does not
+     depend on self-modifying code being possible.
+     The ifence instruction can will flush the instruction cache and therefore put back the
+     set of executable addresses to the whole range.
+     We only store 4-byte aligned addresses, and storeByte has to clear the two low bits. *)
+  Definition XAddrs: Type := list word.
+
+  Definition isXAddrB(a: word)(xAddrs: XAddrs): bool :=
+    match List.find (word.eqb a) xAddrs with
+    | Some _ => true
+    | None => false
+    end.
+
+  Definition isXAddr: word -> XAddrs -> Prop := @List.In word.
+
+  Lemma isXAddrB_holds: forall a xAddrs,
+      isXAddrB a xAddrs = true -> isXAddr a xAddrs.
+  Proof.
+    unfold isXAddrB, isXAddr. intros.
+    destruct (List.find (word.eqb a) xAddrs) eqn: E; [|discriminate].
+    apply List.find_some in E. destruct E.
+    apply Word.Properties.word.eqb_true in H1.
+    subst. assumption.
+  Qed.
+
+  Lemma isXAddrB_not: forall a xAddrs,
+      isXAddrB a xAddrs = false -> ~ isXAddr a xAddrs.
+  Proof.
+    unfold isXAddrB, isXAddr. intros.
+    destruct (List.find (word.eqb a) xAddrs) eqn: E; [discriminate|].
+    intro C.
+    pose proof (List.find_none _ _ E _ C) as P.
+    rewrite Word.Properties.word.eqb_eq in P by reflexivity.
+    discriminate.
+  Qed.
+
+  Lemma isXAddrB_true: forall a xAddrs,
+      isXAddr a xAddrs -> isXAddrB a xAddrs = true.
+  Proof.
+    intros. destruct (isXAddrB a xAddrs) eqn: E; [reflexivity|exfalso].
+    eapply isXAddrB_not; eassumption.
+  Qed.
+
+  Lemma isXAddrB_false: forall a xAddrs,
+      ~ isXAddr a xAddrs -> isXAddrB a xAddrs = false.
+  Proof.
+    intros. destruct (isXAddrB a xAddrs) eqn: E; [exfalso|reflexivity].
+    apply isXAddrB_holds in E. contradiction.
+  Qed.
+
+  Definition removeXAddr(a: word): XAddrs -> XAddrs :=
+    List.filter (fun a' => negb (word.eqb a a')).
+
+  Definition addXAddr: word -> XAddrs -> XAddrs := List.cons.
+
+  Fixpoint addXAddrRange(a: word)(nWords: nat)(xAddrs: XAddrs): XAddrs :=
+    match nWords with
+    | O => xAddrs
+    | S n => addXAddr a (addXAddrRange (word.add a (word.of_Z 4)) n xAddrs)
+    end.
+
   Record RiscvMachine := mkRiscvMachine {
     getRegs: Registers;
     getPc: word;
     getNextPc: word;
     getMem: Mem;
+    getXAddrs: XAddrs;
     getLog: list LogItem;
   }.
 
   Definition withRegs: Registers -> RiscvMachine -> RiscvMachine :=
-    fun regs2 '(mkRiscvMachine regs1 pc nextPC mem log) =>
-                mkRiscvMachine regs2 pc nextPC mem log.
+    fun regs2 '(mkRiscvMachine regs1 pc nextPC mem xAddrs log) =>
+                mkRiscvMachine regs2 pc nextPC mem xAddrs log.
 
   Definition withPc: word -> RiscvMachine -> RiscvMachine :=
-    fun pc2 '(mkRiscvMachine regs pc1 nextPC mem log) =>
-              mkRiscvMachine regs pc2 nextPC mem log.
+    fun pc2 '(mkRiscvMachine regs pc1 nextPC mem xAddrs log) =>
+              mkRiscvMachine regs pc2 nextPC mem xAddrs log.
 
   Definition withNextPc: word -> RiscvMachine -> RiscvMachine :=
-    fun nextPC2 '(mkRiscvMachine regs pc nextPC1 mem log) =>
-                  mkRiscvMachine regs pc nextPC2 mem log.
+    fun nextPC2 '(mkRiscvMachine regs pc nextPC1 mem xAddrs log) =>
+                  mkRiscvMachine regs pc nextPC2 mem xAddrs log.
 
   Definition withMem: Mem -> RiscvMachine -> RiscvMachine :=
-    fun mem2 '(mkRiscvMachine regs pc nextPC mem1 log)  =>
-               mkRiscvMachine regs pc nextPC mem2 log.
+    fun mem2 '(mkRiscvMachine regs pc nextPC mem1 xAddrs log)  =>
+               mkRiscvMachine regs pc nextPC mem2 xAddrs log.
+
+  Definition withXAddrs: XAddrs -> RiscvMachine -> RiscvMachine :=
+    fun xAddrs2 '(mkRiscvMachine regs pc nextPC mem xAddrs1 log)  =>
+                  mkRiscvMachine regs pc nextPC mem xAddrs2 log.
 
   Definition withLog: list LogItem -> RiscvMachine -> RiscvMachine :=
-    fun log2 '(mkRiscvMachine regs pc nextPC mem log1) =>
-               mkRiscvMachine regs pc nextPC mem log2.
+    fun log2 '(mkRiscvMachine regs pc nextPC mem xAddrs log1) =>
+               mkRiscvMachine regs pc nextPC mem xAddrs log2.
 
   Definition withLogItem: LogItem -> RiscvMachine -> RiscvMachine :=
-    fun item '(mkRiscvMachine regs pc nextPC mem log) =>
-               mkRiscvMachine regs pc nextPC mem (item :: log).
+    fun item '(mkRiscvMachine regs pc nextPC mem xAddrs log) =>
+               mkRiscvMachine regs pc nextPC mem xAddrs (item :: log).
 
   Definition withLogItems: list LogItem -> RiscvMachine -> RiscvMachine :=
-    fun items '(mkRiscvMachine regs pc nextPC mem log) =>
-                mkRiscvMachine regs pc nextPC mem (items ++ log).
+    fun items '(mkRiscvMachine regs pc nextPC mem xAddrs log) =>
+                mkRiscvMachine regs pc nextPC mem xAddrs (items ++ log).
 
   Definition Z32s_to_bytes(l: list Z): list byte :=
     List.flat_map (fun z => HList.tuple.to_list (LittleEndian.split 4 z)) l.
@@ -59,6 +127,7 @@ Section Machine.
   Definition putProgram(prog: list MachineInt)(addr: word)(ma: RiscvMachine): RiscvMachine :=
     (withPc addr
     (withNextPc (word.add addr (word.of_Z 4))
-    (withMem (unchecked_store_byte_list addr (Z32s_to_bytes prog) ma.(getMem)) ma))).
+    (withXAddrs (addXAddrRange addr (List.length prog) ma.(getXAddrs))
+    (withMem (unchecked_store_byte_list addr (Z32s_to_bytes prog) ma.(getMem)) ma)))).
 
 End Machine.
